---
output:
  html_document: default
  pdf_document: default
---
# Fourier Series

## Exercise C.1

Let $p \in (0, \pi), \ h \in \mathbb{R}$ and define
\begin{align*}
  f(x) = 
  \begin{cases}
    \dfrac{hx}{p}, &x\in[0,p], \\[2ex]
    \dfrac{h(\pi - x)}{\pi - p}, &x\in(p, \pi].
  \end{cases}
\end{align*}
Show that
\begin{align*}
  f(x) = \sum_{n = 1}^\infty A_n \sin(nx), \quad x\in[o, \pi],
\end{align*}
where
\begin{align*}
  A_n := \frac{2h}{n^2} \frac{\sin(np)}{p(\pi - p)}, \quad n \in \mathbb{N}.
\end{align*}
Convince yourself that $\sum_{n = 1}^\infty |A_n| < \infty$ such that one can utilize theorem C.8.
\newline
\texit{Hint:} You can safe time by expanding $f$ as an uneven function on $[-\pi, \pi]$ and use remark C.4.
\newline
\textbf{Solution:}
\newline
The first thing to do is to expand $f$ as an uneven function.
This is done as follows
\begin{align*}
  \tilde{f}(x) =
  \begin{cases}
    f(x), &x\in[0, \pi] \\[2ex]
    -f(-x), &x\in[-\pi, 0).
  \end{cases}
\end{align*}
Remark C.4 now tells that because $\tilde{f}$ is uneven $a_n(\tilde{f}) = 0$ for all $n\in\mathbb{N}_0$ and
\begin{align*}
  b_n(\tilde{f}) = \frac{2}{l} \int_0^l \sin(n \pi x/l)\tilde{f}(x)\text{d}x, \quad n \in \mathbb{N}.
\end{align*}
With our uneven expansion of $f$ our $b_n(\tilde{f})$ becomes
\begin{align*}
  b_n(\tilde{f}) &= \frac{2}{\pi} \int_0^\pi \sin(n\pi x/\pi) \tilde{f}(x) \ \text{d}x \\
  &= \frac{2}{\pi} \left( \int_0^p \sin(nx)\frac{hx}{p} \ \text{d}x + \int_p^\pi \sin(nx)\frac{h(\pi - x)}{\pi - p} \ \text{d}x \right) \\
  &= \frac{2}{\pi} \left( \frac{h}{p} \int_0^p \sin(nx) x \ \text{d}x + \frac{h}{\pi - p} \int_p^\pi \sin(nx)(\pi - x) \ \text{d}x \right) \\
  &= \frac{2}{\pi} \left( \frac{h}{p} \int_0^p \sin(nx) x \ \text{d}x + \frac{h\pi}{\pi - p} \int_p^\pi \sin(nx) \ \text{d}x - \frac{h}{\pi - p} \int_p^\pi \sin(nx)x \ \text{d}x \right).
\end{align*}
To compute the integrals in the above equation we use partial integration with
\begin{align*}
  f(x) &= x, \qquad &&f'(x) = 1 \\
  g(x) &= \sin(nx), \qquad &&G(x) = -\frac{\cos(nx)}{n},
\end{align*}
and the familiar relation
\begin{align*}
  \int_a^b f(x)g(x) = \left[ f(x)G(x) \right]_a^b + \int_a^b f'(x)G(x) \ \text{d}x.
\end{align*}
This means that the first integral becomes
\begin{align*}
  \int_0^p\sin(nx) x \ \text{d}x &= \left[ -\frac{x\cos(nx)}{n} \right]_0^p - \frac{1}{n} \int_0^p \cos(nx) \ \text{d}x \\
  &= \left[ -\frac{x\cos(nx)}{n} \right]_0^p - \frac{1}{n} \left[ \frac{\sin(nx)}{n} \right]_0^p \\
  &= \left( -\frac{p\cos(np)}{n} - \left[ -\frac{0 \cdot \cos(n \cdot 0)}{n} \right] \right) - \frac{1}{n}\left( \frac{\sin(np)}{n} - \frac{\sin(n \cdot 0)}{n} \right) \\
  &= -\frac{p\cos(np)}{n} - \frac{\sin(np)}{n^2}.
\end{align*}
The second integral becomes
\begin{align*}
  \int_p^\pi \sin(nx) \ \text{d}x &= \left[ -\frac{\cos(nx)}{n} \right]_p^\pi \\
  &= -\frac{\cos(n \pi)}{n} - \left( -\frac{\cos(np)}{n} \right) \\
  &= \frac{1}{n} + \frac{\cos(np)}{n}.
\end{align*}
Lastly the third integral becomes
\begin{align*}
  
\end{align*}